wip on a simpler Handshake state machine, and a separate module for protectiong tickets seals and cookies

src/tls/TLS.Handshake.Machine.fst
@@ -4,7 +4,7 @@ module TLS.Handshake.Machine
 /// monotonic properties, and stateful properties from Transcript,
 /// Negotiation, KeySchedule.
 
-// This is client-only WIP, will replace the start of Old.Handshake.
+// This is client-only WIP, will replace the start of Old.Handshake
 
 open FStar.Error
 open FStar.Bytes // still used for cookies, tickets, signatures... 
@@ -24,39 +24,63 @@ module Transcript = HSL.Transcript
 
 // let Secret = Handshake.Secret
 
-// missing indexes? both elements should be Client-specific, with
-// resumeInfo only for clients.
+// TLS.Config will define a more convenient client-specific configuration
 let client_config = config * Negotiation.resumeInfo 
 
-// Helpful refinement within Secret?
+// Helpful refinement within Secret? stating that an index is for a PSK.
 assume val is_psk: Idx.id -> bool 
 
-// May also depend on the resumeInfo, to be sorted out once we fix the
-// config type.
-assume val psk_ids_of_config: client_config -> list (i:Idx.id{is_psk i})
-assume val groups_of_config: client_config -> list CommonDH.group  
+/// message types (move to HandshakeMessages or Repr modules)
 
-// Offered, depending on first PSK or first ciphersuite.
-// May be overwritten by ServerHello 
-assume val ha_of_offer: Negotiation.offer -> Spec.Hash.Definitions.hash_alg
+type clientHello = HandshakeMessages.clientHello
+type serverHello = HandshakeMessages.serverHello
+type helloRetryRequest = msg: serverHello {Transcript.is_hrr msg} 
+type encryptedExtensions = HandshakeMessages.encryptedExtensions
+type finished = HandshakeMessages.finished // TODO shared type, ideally with tighter bound.
 
-// from Handshake.Secret, currently broken
-assume type secret_c13_wait_ServerHello 
-  (psks  : list (i:_{is_psk i})) 
-  (groups: list CommonDH.group)
+/// To be aligned with Transcript:
+/// retry info, precise for clients, hashed for servers.
 
-// we may need an extra ghost in the implementation of the type above.
-assume val shares_of_ks:
-  #psks  : list (i:_{is_psk i}) ->
-  #groups: list CommonDH.group -> 
-  secret_c13_wait_ServerHello psks groups -> option Extensions.keyShareClientHello
+type client_retry_info = {
+  ch0: clientHello;
+  sh0: helloRetryRequest; }
 
-// will go to Transcript
+type full_offer = {
+  full_retry: option client_retry_info;
+  full_ch: clientHello; // not insisting that ch initially has zeroed binders 
+  }
+
+type offer = { 
+  hashed_retry: option Transcript.retry;
+  ch: clientHello; // not insisting that ch initially has zeroed binders
+  } 
+
 let trans (n:nat) = tr: Transcript.transcript_t { Transcript.transcript_size tr <= n }
 
+// setting binders to some default value determined by the PSK
+// extension; we may need to prove that this function is idempotent
+// and does not affect other accessors.
+assume val clear_binders: clientHello -> clientHello 
 
-// to be adapted in Nego
-assume val nego_find_key_shares: Negotiation.offer -> option Extensions.keyShareClientHello 
+assume val hash_retry: option client_retry_info -> option Transcript.retry
+
+/// To be adapted within Negotation
+/// 
+// Offered, depending on first PSK or first ciphersuite.
+assume val offered_ha:  clientHello -> EverCrypt.Hash.alg
+
+// detail: those two may also return lists
+assume val offered_shares: clientHello -> option Extensions.keyShareClientHello 
+assume val offered_psks: clientHello -> option Extensions.offeredPsks 
+
+/// certificate-based credentials (server-only for now)
+
+assume val selected_ha: serverHello -> EverCrypt.Hash.alg // also applicable to HRR 
+
+type serverCredentials = 
+  option HandshakeMessages.(certificate13 * certificateVerify13) 
+  // where to keep track of the negotiated algorithms? 
+  // at least CertificateVerify could be just a ghost 
 
 val deobfuscate: Negotiation.offer -> Negotiation.resumeInfo -> UInt32.t 
 let deobfuscate offer resumeInfo = 
@@ -70,18 +94,19 @@ let deobfuscate offer resumeInfo =
 // initial offer is a function of the config.
 
 let offered0 ((cfg,resume):client_config) (offer:Negotiation.offer) = 
-  let ks = nego_find_key_shares offer in 
+  let ks = offered_shares offer in 
   let now = deobfuscate offer resume in 
-  Correct offer == Negotiation.client_offer cfg offer.Parsers.ClientHello.random ks resume now 
+  Correct offer == Negotiation.client_offer 
+    cfg offer.Parsers.ClientHello.random ks resume now 
 
-let offered ((cfg,resume):client_config) (prior:option Transcript.retry) (offer:Negotiation.offer) = 
-  match prior with
-  | None -> offered0 (cfg,resume) offer 
-  | Some (digest_ch0, hrr) -> 
-    let ks1 = nego_find_key_shares offer in 
-    let now1 = deobfuscate offer resume in 
-    exists (offer0: Negotiation.offer).
-    offered0 (cfg,resume) offer0 
+let offered ((cfg,resume):client_config) (offer:full_offer) = 
+  let ch = offer.full_ch in 
+  match offer.full_retry with
+  | None -> offered0 (cfg,resume) ch
+  | Some retry -> 
+    let ks1 = offered_shares ch in 
+    let now1 = deobfuscate ch resume in 
+    offered0 (cfg,resume) retry.ch0 
     // TBC Negotiation: /\ 
     // digest_ch0 = hash (selected_hashAlg hrr) offer0 /\ 
     // Correct offer == Negotiation.client_retry cfg offer0 ks now 
@@ -96,6 +121,28 @@ let accepted
   // TBC Negotiation: 
   // missing the late processing of encrypted extensions and its callback. 
 
+assume val accepted13: full_offer -> serverHello -> Type0
+
+assume val client_complete: full_offer -> serverHello -> encryptedExtensions -> serverCredentials -> Type0
+
+
+/// From Handshake.Secret, indexing TBC; for now we omit their
+/// (opaque) part of the state.
+
+assume type secret_c13_wait_ServerHello 
+  (pskis: list (i:_{is_psk i}))
+  (groups: list CommonDH.group) 
+
+// we may need an extra ghost in the implementation of the type above.
+assume val shares_of_ks:
+  #psks  : list (i:_{is_psk i}) ->
+  #groups: list CommonDH.group -> 
+  secret_c13_wait_ServerHello psks groups -> option Extensions.keyShareClientHello
+
+assume val groups_of_ks: 
+  option Extensions.keyShareClientHello -> list CommonDH.group 
+
+assume val pskis_of_psks: option Extensions.offeredPsks -> list (i:_{is_psk i})
 
 
 /// State machine for the connection handshake (private to Handshake).
@@ -104,97 +151,76 @@ let accepted
 /// Low*: we'll turn all high-level messages constructor arguments
 /// into ghost, possibly using reprs.
 
-noeq type client_state  
-  (region:rgn)            // unused for now; worth the trouble? passed only as stateful-invariant argument? 
-  (cfg: client_config)    // duplicating Nego? 
-  (nonce: TLSInfo.random) // could be a function of the transcript, saving one argument? 
-  = 
-
-  // allocation state, initially empty
+noeq type client_state 
+  (region:rgn) // unused for now; worth the trouble? passed only as stateful-invariant argument? 
+  (cfg: client_config) 
+  // removed the nonce (may also be cached)
+=
+  // used only for allocating the client state and binding it to its
+  // local nonce in the connection table.
   | C_init: 
-    client_state region cfg nonce 
+    TLSInfo.random -> 
+    client_state region cfg 
 
-  // intermediate step for witnessing the truncated transcript, 
-  // a pre-condition for the binder HMACs. 
-  // TODO The Transcript state should be TruncatedHello. 
-  | C_truncated_ClientHello: (*
-    retry: _
-    ch : _ 
-    let ha = ... in
-    let transcript = erased (Transcript.ClientHello (Transcript.retry_of retry) (HSM.hsm_of_ch ch)) in 
-    Transcript.digest ha transcript   *)
-    transcript: Ghost.erased (trans 0) -> 
-    offer: Negotiation.offer (* TODO with zeroed binders *) ->
-    digest: Transcript.state (ha_of_offer offer) -> 
-    ks: secret_c13_wait_ServerHello (psk_ids_of_config cfg) (groups_of_config cfg) 
-    { let transcript = Ghost.reveal transcript in 
-      transcript == Transcript.Hello None (HSM.M_client_hello offer) /\
-      ( exists (now:UInt32.t). (Correct offer == Negotiation.client_offer (fst cfg) nonce (shares_of_ks ks) (snd cfg) now)) }
-    -> 
-    client_state region cfg nonce 
+  // waiting for ServerHello (1.3) or ServerHello...ServerHelloDone
+  // (1.2); this state may be updated after receiving HRR; it is also
+  // used (transiently) for witnessing the pre-condition of the binder
+  // HMACs, before providing the actual binders; the Handshake
+  // invariant (specifying the Transcript state) does not hold in that
+  // intermediate state.
+  | C_wait_ServerHello:
+    offer: full_offer { offered cfg offer } -> 
+    // Witnessed in the binders, then overwritten to add binders or
+    // a retry. 
 
-  // waiting for plaintext ServerHello.
-  | C_wait_ServerHello: 
-    transcript: Ghost.erased (trans 0) -> 
-    offer: Negotiation.offer -> 
-    digest: Transcript.state (ha_of_offer offer) -> 
-    ks: secret_c13_wait_ServerHello (psk_ids_of_config cfg) (groups_of_config cfg) 
-    { let transcript = Ghost.reveal transcript in 
-      transcript == Transcript.Hello None (HSM.M_client_hello offer) /\
-      //Negotiation.correct_client_offer nego cfg nonce (shares_of_ks ks) resume now
-      ( exists (now:UInt32.t). (Correct offer == Negotiation.client_offer (fst cfg) nonce (shares_of_ks ks) (snd cfg) now))
-      } -> 
-    client_state region cfg nonce 
+    digest: Transcript.state (offered_ha offer.full_ch) (* ..tch then ..ch *) -> 
+    // typically re-used, unless the serve pick another algorithm
+    ks: secret_c13_wait_ServerHello 
+      (pskis_of_psks (offered_psks offer.full_ch)) 
+      (groups_of_ks (offered_shares offer.full_ch)) ->
+    // keeping the associated infos, master secrets, and exponents
+    client_state region cfg  
 
-  // waiting for encrypted handshake (1.3 only)
+  // waiting for encrypted handshake (1.3 only). The optional binders
+  // are now ghost, and the transcript now uses the hash algorithm
+  // chosen by the server. We may need to add a C13_sent_EOED variant.
   | C13_wait_Finished1: 
-    transcript: Ghost.erased (trans 1) -> 
-    nego: Negotiation.mode ->
-    digest: Transcript.state (Negotiation.hashAlg nego) 
-    { let transcript = Ghost.reveal transcript in
-      let offer = nego.Negotiation.n_offer in (
-      exists (sh:_) (now:UInt32.t) (shares:_). 
-      Correct offer == Negotiation.client_offer (fst cfg) nonce shares (snd cfg) now /\
-      Correct nego == Negotiation.accept_ServerHello (fst cfg) offer sh /\ 
-      Transcript.nego_version (HSM.M_client_hello offer) (HSM.M_server_hello sh) == TLS_1p3 /\ 
-      transcript == Transcript.Transcript13 
-        None (HSM.M_client_hello offer) (HSM.M_server_hello sh) [] )
-    }                                 
-    -> 
+    offer: full_offer{ offered cfg offer } -> 
+
+    sh: serverHello{ accepted13 offer sh (* not yet authenticated *) } -> 
+    digest: Transcript.state (selected_ha sh) (* ..sh, now using the server's ha *) -> 
+    // TODO key-schedule state 
     //i:   Secret.hs_id ->
     //ams: Secret.ams (Secret.ams_of_hms i) ->
     //cfk: Secret.fink (Secret.cfk_of_hms i) ->
     //sfk: Secret.fink (Secret.sfk_of_hms i) -> 
-    client_state region cfg nonce 
+    client_state region cfg 
 
-  // waiting for post-handshake messages (1.3 only; TBC rekeying)
-  // this state is witnessed to produce Finished2, 
-  // hencee it does not include it in the transcript. 
-  | C13_complete: 
-    transcript: Ghost.erased (trans 5) -> 
-    nego: Negotiation.mode -> 
-    digest: Transcript.state (Negotiation.hashAlg nego)
-    { let transcript = Ghost.reveal transcript in 
-      let offer = nego.Negotiation.n_offer in (
-      exists 
-        (now:UInt32.t) 
-        (shares:_)
-        (sh:_) (ee:_) (* we care about their contributions to the negotiated mode *)
-        (fin:_)       (* ignored once verified *) 
-        .
-      Correct offer == Negotiation.client_offer (fst cfg) nonce shares (snd cfg) now /\
-      Correct nego == Negotiation.accept_ServerHello (fst cfg) offer sh /\ 
-      Transcript.nego_version (HSM.M_client_hello offer) (HSM.M_server_hello sh) == TLS_1p3 /\ 
-      transcript == Transcript.Transcript13 
-        None (HSM.M_client_hello offer) (HSM.M_server_hello sh) 
-        [ Parsers.Handshake13.M13_encrypted_extensions ee; 
-          Parsers.Handshake13.M13_finished fin ] )
-      // TBC experiment with branching abstraction? 
-    }
-    -> 
-    //i:   Secret.ams_id ->
-    //rms: Secret.secret (rms_of_ams i tr) (* for accepting resumption tickets *) ->
-    client_state region cfg nonce 
+  // waiting for post-handshake messages (1.3 only; TBC rekeying);
+  // also used for witnessing the pre-condition of the client finished
+  // HMAC (and the client signature TBC) in which case fin2 is not yet
+  // set & included in the transcript; we also remain in that state as
+  // we receive tickets.
+  | C13_complete:
+    offer: full_offer{ offered cfg offer } -> 
+    sh: serverHello{ accepted13 offer sh } -> 
+    digest: Transcript.state (selected_ha sh) (* ..fin1 then ..fin2 *) -> 
+
+    ee: encryptedExtensions -> 
+    server_id: serverCredentials ->
+    fin1: Ghost.erased finished -> (* received from the server *) 
+    fin2: Ghost.erased finished (* sent by the client *) 
+    // We keep the finished messages only to specify the transcript digest.
+    { client_complete offer sh ee server_id } -> 
+//  i:   Secret.ams_id ->
+//  rms: Secret.secret (rms_of_ams i tr) (* for accepting resumption tickets *) ->
+    client_state region cfg  
+
+    // let client_complete offer sh ee svn = 
+    //   client_offered cfg offer /\ 
+    //   client_accepted13 offer sh /\ 
+    //   client_verified13 offer sh ee svc /\ 
+    //   (honest_server sh ... ==> server_selected13 offer sh ee svc) 
 
 
 (*
@@ -230,26 +256,29 @@ noeq type client_state
 // we embed in the type above refinements for functional properties
 // and witnessed properties, but we also need a stateful invariant.
 
+
 let client_invariant 
   (#region:rgn) (#cfg: client_config) (#nonce: TLSInfo.random) 
-  (state: client_state region cfg nonce)
+  (state: client_state region cfg)
   (h: HS.mem) 
 = 
   match state with 
-  | C_init -> True
+  | C_init _ -> True 
 
-  | C_truncated_ClientHello transcript offer digest ks 
-  | C_wait_ServerHello transcript offer digest ks -> 
-    let transcript = Ghost.reveal transcript in 
+  | C_wait_ServerHello offer digest ks -> 
+
+    let transcript = Transcript.ClientHello (hash_retry offer.full_retry) offer.full_ch in 
+    // let transcript = Ghost.reveal transcript in 
     Transcript.invariant digest transcript h
     // Secret.invariant ks h
 
-  | C13_wait_Finished1 transcript mode digest ->
-    let transcript = Ghost.reveal transcript in 
+  | C13_wait_Finished1 offer sh digest  ->
+    let sh : _ = assume False; sh in // mismatch on transcript refinement   
+    let transcript = Transcript.Transcript13 (hash_retry offer.full_retry) offer.full_ch sh [] in
     Transcript.invariant digest transcript h
     // Secret.invariant_C13_wait_Finished1 ks
+
   | _ -> False 
-  
 
 /// We define an update condition on the state that encodes the state
 /// machine and ensures stability on selected properties of
@@ -257,110 +286,249 @@ let client_invariant
 /// Negotiation's offer and mode are SSA.
 
 let step
-  (#region:rgn) (#cfg: client_config) (#nonce: TLSInfo.random)
-  (st0 st1: client_state region cfg nonce)
+  (#region:rgn) (#cfg: client_config) 
+  (st0 st1: client_state region cfg)
 = //st0 == undo_last_step st1 
   match st0, st1 with 
 
   // | Cn x, Cn' x' y' -> x == x'  
-  | C_init,
-    C_truncated_ClientHello transcript0 offer0 digest0 ks0 -> True
+  | C_init nonce0,
+    C_wait_ServerHello offer1 digest1 ks1 -> offer1.full_ch.Parsers.ClientHello.random == nonce0
 
-  | C_truncated_ClientHello transcript0 offer0 digest0 ks0,
-    C_wait_ServerHello      transcript1 offer1 digest1 ks1 ->
-    let transcript0 = Ghost.reveal transcript0 in 
-    let transcript1 = Ghost.reveal transcript1 in 
-    exists (binders:_). 
-    Some transcript1 == Transcript.transition_hsm transcript0 binders /\
-    //19-05-15 can we avoid the option? 
+  | C_wait_ServerHello offer0 digest0 ks0,
+    C_wait_ServerHello offer1 digest1 ks1 ->
+    // enabling addition of the real binders
+    ( offer0.full_retry == offer1.full_retry /\
+      clear_binders offer0.full_ch == clear_binders offer1.full_ch)  \/
+    // enabling addition of a retry; too lax for now 
+    ( match offer0.full_retry, offer1.full_retry with 
+      | None, Some hr -> hr.ch0 = offer0.full_ch 
+      | _ -> False )
+
+  | C_wait_ServerHello offer0 digest0 ks0,
+    C13_wait_Finished1 offer1 sh1 digest1 -> 
+    offer1 == offer0
     
-    True //offer1 == transcript_offer transcript1 
-
-  | C_wait_ServerHello      transcript0 offer0 digest0 ks0,
-    C13_wait_Finished1      transcript1 mode1 digest1 ->
-    let transcript0 = Ghost.reveal transcript0 in 
-    let transcript1 = Ghost.reveal transcript1 in (
-    exists (sh:_). 
-    Some transcript1 == Transcript.transition_hsm transcript0 sh )
-
   | _, _ -> False 
 
-// sample lemma: the offer is SSA. 
-
-let st_offer
-  (#region:rgn) (#cfg: client_config) (#nonce: TLSInfo.random)
-  (st0: client_state region cfg nonce) 
-= 
-  match st0 with 
-  | C_wait_ServerHello transcript0 offer0 digest0 ks0 -> Some offer0 
-  | C13_wait_Finished1 transcript0 mode0 digest0 -> Some mode0.Negotiation.n_offer
-  | _ -> None 
-
-let m_offer 
-  (#region:rgn) (#cfg: client_config) (#nonce: TLSInfo.random)
-  (st0 st1: client_state region cfg nonce):
-  Lemma (
-    let o0 = st_offer st0 in
-    let o1 = st_offer st1 in
-    step st0 st1 /\ Some? o0 ==> o1 == o0)
-=
-  ()
-
 let mrel 
-  (#region:rgn) (#cfg: client_config) (#nonce: TLSInfo.random)
-= ReflexiveTransitiveClosure.closure (step #region #cfg #nonce)
+  (#region:rgn) (#cfg: client_config) =
+  FStar.ReflexiveTransitiveClosure.closure (step #region #cfg)
 
-/// Main type for the connection handshake
+/// We can finally define our main, stateful, monotonic type for the connection handshake
 noeq abstract type t (region:rgn) = {
   cfg: client_config;
   nonce: TLSInfo.random;
   state: st:HST.mreference 
-    (client_state region cfg nonce) 
-    (mrel #region #cfg #nonce) 
+    (client_state region cfg) 
+    (mrel #region #cfg) 
     { HS.frameOf st = region } }
 
-/// Testing monotonicity, thanks to the new closure library
 
-let p #region (st:t region) (o:Negotiation.offer) h0 = 
-  st_offer (HS.sel h0 st.state) == Some o 
+/// ----------------------------------------------------------------
+/// sample SSA properties: the initial and retried ClientHello
+/// messages are both stable once defined, except for their binders.
 
-val witness_offer (#region:rgn) (st:t region): 
-  Stack 
-    (o: Negotiation.offer{ token_p st.state (p st o) })
+(* Together with transcript injectivity, this is the gist of the
+   authentication carried by the binders, of the form 
+
+fun m -> 
+  forall transcript.
+  m = transcript_hash transcript ==>
+  match transcript with
+   | TruncatedClientHello retried tch ->
+       let crandom = client_random tch in
+       token_p (
+         fun h0 -> 
+         match client_lookup h0 crandom with  
+         | None -> False // there is a honest client such that ...
+         | Some (cfg & st) ->  
+           match retried with
+           | None    -> token_ch0 st tch
+           | Some hr -> token_ch0 st hr.ch0 /\ token_ch1 st tch )
+
+   | _ -> False // no other messages are MACed with the binder key.
+*)
+
+let st_ch0 (#region:rgn) (#cfg: client_config) (st: client_state region cfg) =
+  match st with 
+  | C_init _ -> None 
+  | C_wait_ServerHello offer _ _  
+  | C13_wait_Finished1 offer _ _ 
+  | C13_complete offer _ _ _ _ _ _ -> 
+    match offer.full_retry with 
+    | None    -> Some (clear_binders offer.full_ch)
+    | Some hr -> Some (clear_binders hr.ch0)
+
+let st_ch1 (#region:rgn) (#cfg: client_config) (st: client_state region cfg) =
+  match st with 
+  | C_init _ -> None 
+  | C_wait_ServerHello offer _ _  
+  | C13_wait_Finished1 offer _ _ 
+  | C13_complete offer _ _ _ _ _ _ -> 
+    match offer.full_retry with 
+    | None    -> None 
+    | Some _  -> Some (clear_binders offer.full_ch)
+
+// as a counter-example, this property is not stable:
+let st_ch (#region:rgn) (#cfg: client_config) (st: client_state region cfg) =
+  match st with 
+  | C_init _ -> None 
+  | C_wait_ServerHello offer _ _  
+  | C13_wait_Finished1 offer _ _ 
+  | C13_complete offer _ _ _ _ _ _ -> 
+    Some (clear_binders offer.full_ch)
+
+// establishing their stability for every step; to trivial to apply
+// below, but apparently not required.
+let ssa f st0 st1 = Some? (f st0) ==> f st0 == f st1 
+
+let st_mon 
+  (f: (#region:rgn -> #cfg: client_config -> client_state region cfg -> _)) = 
+  region:rgn -> cfg: client_config -> 
+  st0:client_state region cfg ->
+  st1:client_state region cfg -> Lemma (step st0 st1 ==> ssa f st0 st1)
+  
+let m_ch0: st_mon st_ch0 = fun _ _ _ _ -> () 
+let m_ch1: st_mon st_ch1 = fun _ _ _ _ -> () 
+// expected to fail
+//let m_ch: st_mon st_ch = fun _ _ _ _ -> () 
+
+/// Testing monotonicity, relying on the new closure library; we could
+/// probably do it more parametrically to scale up.
+
+let p #region (st:t region) f (o:Negotiation.offer) h0 = 
+  f (HS.sel h0 st.state) == Some o 
+
+val witness0 (#region:rgn) (st: t region):  
+  Stack clientHello 
     (requires fun h0 -> 
       h0 `HS.contains` st.state /\
-      (match HS.sel h0 st.state with 
-      | C_wait_ServerHello _ _ _ _ 
-      | C13_wait_Finished1 _ _ _ -> True
-      | _ -> False ))
-    (ensures fun h0 o h1 -> modifies_none h0 h1)
-
-let witness_offer #region st =
-  match st_offer !st.state with 
+      ( match HS.sel h0 st.state with 
+        | C_init _ -> False
+        | _        -> True ))
+    (ensures fun h0 o h1 -> 
+      token_p st.state (p st st_ch0 o) /\
+      modifies_none h0 h1)
+      
+let witness0 #region st =
+  match st_ch0 !st.state with 
   | Some o -> (
       ReflexiveTransitiveClosure.stable_on_closure 
-        (step #region #st.cfg #st.nonce) 
-        (fun st -> st_offer st == Some o) ();         
-      witness_p st.state (p st o);
+        (step #region #st.cfg) 
+        (fun st -> st_ch0 st == Some o) ();         
+      witness_p st.state (p #region st st_ch0 o);
       o )
 
+val witness1 (#region:rgn) (st: t region):  
+  Stack clientHello 
+    (requires fun h0 -> 
+      h0 `HS.contains` st.state /\
+      ( match HS.sel h0 st.state with 
+        | C_init _ -> False
+        | C_wait_ServerHello offer _ _  
+        | C13_wait_Finished1 offer _ _ 
+        | C13_complete offer _ _ _ _ _ _ -> Some? offer.full_retry ))
+    (ensures fun h0 o h1 -> 
+      token_p st.state (p st st_ch1 o) /\
+      modifies_none h0 h1)
+      
+let witness1 #region st =
+  match st_ch1 !st.state with 
+  | Some o -> (
+      ReflexiveTransitiveClosure.stable_on_closure 
+        (step #region #st.cfg) 
+        (fun st -> st_ch1 st == Some o) ();         
+      witness_p st.state (p #region st st_ch1 o);
+      o )
 
-(* TODO server-side
-  | S_Idle
+assume val stuff (#region:rgn) (st: t region): Stack unit 
+  (requires fun h0      -> h0 `HS.contains` st.state)
+  (ensures  fun h0 _ h1 -> h1 `HS.contains` st.state)
+  
+let test (#region:rgn) (st: t region): 
+  Stack unit 
+    (requires fun h0 -> h0 `HS.contains` st.state)
+    (ensures fun h0 _ h1 -> True) 
+=
+  let r = st_ch1 !st.state in 
+  if Some? r then 
+    let o = witness1 st in 
+    stuff st; 
+    let r' = st_ch1 !st.state in 
+    recall_p st.state (p st st_ch1 o);
+    assert(r' == Some o)
 
-  | S13_sent_ServerHello:      // TLS 1.3, intermediate state to encryption
-    i: Idx.id -> // Secret.esId ->
-    idh: Idx.id_dhe ->
-    ks: Secret.s13_wait_ServerHello i idh -> machineState
+/// -------------end of sanity check----------------
 
 
-  | S_wait_EOED                // Waiting for EOED
-  | S_wait_Finished2 of digest // TLS 1.3, digest to be MACed by client
-  | S_wait_CCS1                // TLS classic
-  | S_wait_Finished1 of digest // TLS classic, digest to the MACed by client
-  | S_wait_CCS2 of digest      // TLS resume (CCS)
-  | S_wait_CF2 of digest       // TLS resume (CF)
-  | S_Complete
-*) 
+(* the server side is WIP 
+
+type server_retry_info = digest0: bytes & helloRetryRequest
+type s_offer = {
+  retry: option retry_server_info;
+  ch: clientHello; }
+
+// Complete mode for the connection; sufficient to derive all the
+// negotiated connection parameters, and shared between clients and
+// servers when the connection is safe. 
+// 
+// As a technicality, it includes only the *tag* supposed to be the
+// hash of the initial offer after a retry.
+
+type s13_mode (region:rgn) (cfg:server_config) = {
+  offer: s_offer; (* { honest_psk offer ==> client_offered offer } *) 
+  sh: serverHello; 
+  ee: encryptedExtensions;
+  certs: certs:option HandshakeMessage.certificate13
+  { 
+    // including the nego callback that led to those choices; we may want to keep its [cfg']
+    selected cfg offer sh ee certs };
+  }
+  
+
+type server_state 
+  (region:rgn)
+  (cfg: server_config) // much smaller than before
+=  
+
+  | S_wait_ClientHello:
+    server_state rgn cfg 
+
+  // TLS 1.3, intermediate state to encryption
+  | S13_sent_ServerHello:      
+    mode: s13_mode -> 
+    digest: Transcript.state (selected_ha sh) -> 
+//  i: Idx.id -> // Secret.esId ->
+//  idh: Idx.id_dhe ->
+//  ks: Secret.s13_wait_ServerHello i idh -> 
+    server_state region cfg 
+
+//// TLS 1.3 intermediate state
+//| S13_wait_EOED 
+
+  | S13_wait_Finished2:
+    mode: s13_mode -> 
+    digest: Transcript.state (selected_ha sh) (* expected to be MACed in the Client Finished *) -> 
+    ssv: Ghost.erased HandshakeMessages.certificateVerify13 ->  
+    fin1: Ghost.erased finished ->
+//  ks: keeping fin2key and rms   
+    server_state region cfg 
+
+  | S13_complete: 
+    mode: s13_mode -> 
+    ssv: Ghost.erased HandshakeMessages.certificateVerify13 ->  
+    fin1: Ghost.erased finished ->
+    fin2: Ghost.erased finished 
+    { client_complete mode } -> 
+//  ks: keeping rms    
+    server_state region cfg 
 
 
+//| S_wait_CCS1                // TLS classic
+//| S_wait_Finished1 of digest // TLS classic, digest to the MACed by client
+//| S_wait_CCS2 of digest      // TLS resume (CCS)
+//| S_wait_CF2 of digest       // TLS resume (CF)
+//| S_Complete
+
+*)
